Anh's proof

shiftreset/shift_reset.v
@@ -23,6 +23,18 @@ Fixpoint type_denote (t : type) : Type :=
   | TyFunc dom ran a b => type_denote dom -> (type_denote ran -> type_denote a) -> type_denote b
   end.
 
+Lemma fold_unfold_type_denote_TyPure :
+  forall (t : Type),
+    type_denote (TyPure t) =
+    t.
+Proof. auto. Qed.
+
+Lemma fold_unfold_type_denote_TyFunc :
+  forall (dom ran a b : type),
+    type_denote (TyFunc dom ran a b) =
+    (type_denote dom -> (type_denote ran -> type_denote a) -> type_denote b).
+Proof. auto. Qed.
+
 (** [x : Expr t a b] means that the term [x] has type [t] and evaluation of it changes the answer type from [a] to [b]. *)
 Definition Expr t a b := forall var, expr var t a b.
 
@@ -55,20 +67,102 @@ Defined.
 Definition interpret (t : type) (e : expr type_denote t t t) : type_denote t :=
   interpret_aux t t t e (fun x => x).
 
+Lemma fold_unfold_interpret_aux_Var :
+  forall (t a : type)
+         (x : type_denote t)
+         (k : type_denote t -> type_denote a),
+    interpret_aux t a a (Var type_denote t a x) k =
+    k x.
+Proof. auto. Qed.
+
+Lemma fold_unfold_interpret_aux_Const :
+  forall (t : Type)
+         (a : type)
+         (v : t)
+         (k : t -> type_denote a),
+    interpret_aux (TyPure t) a a (Const type_denote t a v) k =
+    k v.
+Proof. auto. Qed.
+
+Lemma fold_unfold_interpret_aux_Abs :
+  forall (dom ran a b c : type)
+         (f : type_denote dom -> expr type_denote ran a b)
+         (k : (type_denote dom -> (type_denote ran -> type_denote a) -> type_denote b) -> type_denote c),
+    interpret_aux (TyFunc dom ran a b) c c (Abs type_denote dom ran a b c f) k =
+    k (fun x => interpret_aux ran a b (f x)).
+Proof. auto. Qed.
+
+Lemma fold_unfold_interpret_aux_App :
+  forall (dom ran a b c d : type)
+         (e1 : expr type_denote (TyFunc dom ran a b) c d)
+         (e2 : expr type_denote dom b c)
+         (k : type_denote ran -> type_denote a),
+    interpret_aux ran a d (App type_denote dom ran a b c d e1 e2) k =
+    interpret_aux (TyFunc dom ran a b) c d e1 (fun f => interpret_aux dom b c e2 (fun x => f x k)).
+Proof. auto. Qed.
+
+Lemma fold_unfold_interpret_aux_Lift :
+  forall (dom ran : Type)
+         (a b : type)
+         (f : dom -> ran)
+         (e : expr type_denote (TyPure dom) a b)
+         (k : ran -> type_denote a),
+    interpret_aux (TyPure ran) a b (Lift type_denote dom ran a b f e) k =
+    interpret_aux (TyPure dom) a b e (fun x => k (f x)).
+Proof. auto. Qed.
+
+Lemma fold_unfold_interpret_aux_Shift :
+  forall (t a b c d : type)
+         (f : (type_denote t -> (type_denote a -> type_denote d) -> type_denote d) -> expr type_denote c c b)
+         (k : type_denote t -> type_denote a),
+    interpret_aux t a b (Shift type_denote t a b c d f) k =
+    interpret_aux c c b (f (fun x k' => k' (k x))) (fun x => x).
+Proof. auto. Qed.
+
+Lemma fold_unfold_interpret_aux_Reset :
+  forall (t a b : type)
+         (e : expr type_denote a a t)
+         (k : type_denote t -> type_denote b),
+    interpret_aux t b b (Reset type_denote t a b e) k =
+    k (interpret_aux a a t e (fun x => x)).
+Proof. auto. Qed.
+
 Require Import List Arith.
 Import ListNotations.
 
-Fixpoint append_delim_aux (A : Type) (xs : list A) :=
+Fixpoint append_delim_aux (A : Type) (xs : list A) :
+  expr type_denote
+    (TyPure (list A))
+    (TyPure (list A))
+    (TyFunc (TyPure (list A)) (TyPure (list A)) (TyPure (list A)) (TyPure (list A))) :=
   match xs with
-  | [] => Shift type_denote _ _ _ _ (TyPure (list A)) (fun k => Var _ _ _ k)
-  | x :: xs' => Lift _ _ _ (TyPure (list A)) _ (cons x) (append_delim_aux A xs')
+  | [] => Shift _ _ _ _ _ _ (fun k => Var _ _ _ k)
+  | x :: xs' => Lift _ _ _ _ _ (cons x) (append_delim_aux A xs')
   end.
 
-Definition append_delim (A : Type) (xs ys : list A) : list A :=
-  interpret _ (App _ _ _ _ _ _ _ (Reset _ _ _ _ (append_delim_aux A xs)) (Const _ _ _ ys)).
+Lemma fold_unfold_append_delim_aux_nil :
+  forall (A : Type),
+    append_delim_aux A [] =
+    Shift _ _ _ _ _ _ (fun k => Var _ _ _ k).
+Proof. auto. Qed.
+
+Lemma fold_unfold_append_delim_aux_cons :
+  forall (A : Type)
+         (x : A)
+         (xs' : list A),
+    append_delim_aux A (x :: xs') =
+    Lift _ _ _ _ _ (cons x) (append_delim_aux A xs').
+Proof. auto. Qed.
+
+Definition append_delim (A : Type) (xs ys : list A) :
+  expr type_denote
+    (TyPure (list A))
+    (TyPure (list A))
+    (TyPure (list A)) :=
+  App _ _ _ _ _ _ _ (Reset _ _ _ _ (append_delim_aux A xs)) (Const _ _ _ ys).
 
 Definition append_delim_unit_tests : bool :=
-  let unit_test xs ys := if list_eq_dec Nat.eq_dec (append_delim nat xs ys) (xs ++ ys) then true else false in
+  let unit_test xs ys := if list_eq_dec Nat.eq_dec (interpret _ (append_delim nat xs ys)) (xs ++ ys) then true else false in
   unit_test [] []
   && unit_test [] [0]
   && unit_test [0] []
@@ -81,18 +175,149 @@ Definition append_delim_unit_tests : bool :=
 
 Compute append_delim_unit_tests.
 
-Lemma append_delim_base: forall (A:Type) ys,
-  append_delim A [] ys = ys.
-Proof.
-  intros.
-  unfold append_delim.
-  simpl.
-Admitted.
+Lemma fold_unfold_app_nil :
+  forall (A : Type)
+         (ys : list A),
+    [] ++ ys = ys.
+Proof. auto. Qed.
 
-Lemma append_delim_correct: forall (A:Type) xs ys,
-  append_delim A xs ys = xs ++ ys.
+Lemma fold_unfold_app_cons :
+  forall (A : Type)
+         (x : A)
+         (xs ys : list A),
+    (x :: xs) ++ ys = x :: xs ++ ys.
+Proof. auto. Qed.
+
+Lemma append_delim_is_equivalence_to_append_aux :
+  forall (A : Type)
+         (xs ys : list A)
+         (k : list A -> list A),
+    interpret_aux
+      (TyPure (list A))
+      (TyPure (list A))
+      (TyFunc (TyPure (list A)) (TyPure (list A)) (TyPure (list A)) (TyPure (list A)))
+      (append_delim_aux A xs) k ys (fun x => x) =
+    k (xs ++ ys).
 Proof.
-  intros A xs. induction xs; intros.
-  { simpl.
-    apply append_delim_base. }
-Abort.
+  intros A xs ys.
+  induction xs as [| x xs' IHxs']; intros k.
+  - rewrite -> fold_unfold_append_delim_aux_nil.
+    rewrite -> fold_unfold_interpret_aux_Shift.
+    rewrite -> fold_unfold_interpret_aux_Var.
+    rewrite -> app_nil_l.
+    reflexivity.
+  - rewrite -> fold_unfold_append_delim_aux_cons.
+    rewrite -> fold_unfold_interpret_aux_Lift.
+    rewrite -> fold_unfold_app_cons.
+    rewrite -> (IHxs' (fun r : type_denote (TyPure (list A)) => k (x :: r))).
+    reflexivity.
+Qed.
+
+Theorem append_delim_is_equivalence_to_append :
+  forall (A : Type)
+         (xs ys : list A),
+    interpret (TyPure (list A)) (append_delim A xs ys) =
+    xs ++ ys.
+Proof.
+  intros A xs ys.
+  unfold interpret, append_delim.
+  rewrite -> fold_unfold_interpret_aux_App.
+  rewrite -> fold_unfold_interpret_aux_Reset.
+  rewrite -> fold_unfold_interpret_aux_Const.
+  exact (append_delim_is_equivalence_to_append_aux A xs ys (fun x => x)).
+Qed.
+
+Fixpoint times_delim_aux (xs : list nat) :
+  expr type_denote
+    (TyPure nat)
+    (TyPure nat)
+    (TyPure nat) :=
+  match xs with
+  | [] => Const _ _ _ 1
+  | x :: xs' => match x with
+                | O => Shift _ _ _ _ _ (TyPure nat) (fun _ => Const _ _ _ 0)
+                | _ => Lift _ _ _ _ _ (Nat.mul x) (times_delim_aux xs')
+                end
+  end.
+
+Definition times_delim (xs : list nat) :
+  expr type_denote
+    (TyPure nat)
+    (TyPure nat)
+    (TyPure nat) :=
+  Reset _ _ _ _ (times_delim_aux xs).
+
+Lemma fold_unfold_times_delim_aux_nil :
+  times_delim_aux [] =
+  Const _ _ _ 1.
+Proof. auto. Qed.
+
+Lemma fold_unfold_times_delim_aux_cons :
+  forall (x : nat)
+         (xs' : list nat),
+    times_delim_aux (x :: xs') =
+    match x with
+    | O => Shift _ _ _ _ _ (TyPure nat) (fun _ => Const _ _ _ 0)
+    | _ => Lift _ _ _ _ _ (Nat.mul x) (times_delim_aux xs')
+    end.
+Proof. auto. Qed.
+
+Fixpoint times (xs : list nat) : nat :=
+  match xs with
+  | [] => 1
+  | x :: xs' => x * times xs'
+  end.
+
+Lemma fold_unfold_times_nil :
+  times [] = 1.
+Proof. auto. Qed.
+
+Lemma fold_unfold_times_cons :
+  forall (x : nat)
+         (xs' : list nat),
+    times (x :: xs') =
+    x * times xs'.
+Proof. auto. Qed.
+
+Lemma times_delim_is_equivalence_to_times_aux :
+  forall (xs : list nat)
+         (k : nat -> nat),
+    interpret_aux (TyPure nat) (TyPure nat) (TyPure nat) (times_delim_aux xs) k =
+    match times xs with
+    | O => O
+    | S r' => k (S r')
+    end.
+Proof.
+  intros xs.
+  induction xs as [| x xs' IHxs']; intros k.
+  - rewrite -> fold_unfold_times_delim_aux_nil.
+    rewrite -> fold_unfold_interpret_aux_Const.
+    rewrite -> fold_unfold_times_nil.
+    reflexivity.
+  - rewrite -> fold_unfold_times_delim_aux_cons.
+    rewrite -> fold_unfold_times_cons.
+    destruct x as [| x'].
+    + rewrite -> fold_unfold_interpret_aux_Shift.
+      rewrite -> fold_unfold_interpret_aux_Const.
+      reflexivity.
+    + rewrite -> fold_unfold_interpret_aux_Lift.
+      rewrite -> (IHxs' (fun r : type_denote (TyPure nat) => k (S x' * r))).
+      destruct (times xs') as [| r'].
+      * rewrite -> Nat.mul_0_r.
+        reflexivity.
+      * reflexivity.
+Qed.
+
+Theorem times_delim_is_equivalence_to_times :
+  forall (xs : list nat),
+    interpret (TyPure nat) (times_delim xs) =
+    times xs.
+Proof.
+  intros xs.
+  unfold interpret, times_delim.
+  rewrite -> fold_unfold_interpret_aux_Reset.
+  assert (ly := times_delim_is_equivalence_to_times_aux xs (fun x => x)).
+  destruct (times xs) as [| r'].
+  - exact ly.
+  - exact ly.
+Qed.
